Share some more type abbreviations. More code reduction. Blocked on an unidentified issue.

code/curve25519/Hacl.Curve25519_51.fst
@@ -6,6 +6,9 @@ open Hacl.Meta.Curve25519
 // The Hacl core.
 module C = Hacl.Impl.Curve25519.Field51
 
+let g25519: g25519_t =
+  Lib.Buffer.createL_global Spec.Curve25519.basepoint_list
+
 #set-options "--max_fuel 0 --max_ifuel 0 --z3rlimit 100"
 let point_add_and_double =
   addanddouble_point_add_and_double_higher #M51 C.fmul C.fsqr2 C.fmul1 C.fmul2 C.fsub C.fadd
@@ -17,6 +20,5 @@ let fsquare_times = finv_fsquare_times_higher #M51 C.fsqr
 let finv = finv_finv_higher #M51 fsquare_times C.fmul
 let encode_point = generic_encode_point_higher #M51 C.store_felem C.fmul finv
 let scalarmult = generic_scalarmult_higher #M51 encode_point montgomery_ladder decode_point
-let secret_to_public = generic_secret_to_public_higher #M51 scalarmult
+let secret_to_public = generic_secret_to_public_higher #M51 scalarmult g25519
 let ecdh = generic_ecdh_higher #M51 scalarmult
-
