code/curve25519/Hacl.Curve25519_64_Slow.fsti
@@ -1,47 +1,8 @@
 module Hacl.Curve25519_64_Slow
 
-open FStar.HyperStack
-open FStar.HyperStack.All
-
-open Lib.IntTypes
-open Lib.Buffer
-
-open Hacl.Impl.Curve25519.Fields
 open Hacl.Impl.Curve25519.Generic
+open Hacl.Impl.Curve25519.Fields
 
-module S = Spec.Curve25519
-
-val scalarmult:
-    shared:lbuffer uint8 32ul
-  -> my_priv:lbuffer uint8 32ul
-  -> their_pub:lbuffer uint8 32ul
-  -> Stack unit
-    (requires fun h0 ->
-      Vale.X64.CPU_Features_s.(adx_enabled /\ bmi2_enabled) /\
-      live h0 shared /\ live h0 my_priv /\ live h0 their_pub /\
-      disjoint shared my_priv /\ disjoint shared their_pub)
-    (ensures  fun h0 _ h1 -> modifies (loc shared) h0 h1 /\
-      as_seq h1 shared == S.scalarmult (as_seq h0 my_priv) (as_seq h0 their_pub))
-
-val secret_to_public:
-    pub:lbuffer uint8 32ul
-  -> priv:lbuffer uint8 32ul
-  -> Stack unit
-    (requires fun h0 ->
-      Vale.X64.CPU_Features_s.(adx_enabled /\ bmi2_enabled) /\
-      live h0 pub /\ live h0 priv /\ disjoint pub priv)
-    (ensures  fun h0 _ h1 -> modifies (loc pub) h0 h1 /\
-      as_seq h1 pub == S.secret_to_public (as_seq h0 priv))
-
-val ecdh:
-    shared:lbuffer uint8 32ul
-  -> my_priv:lbuffer uint8 32ul
-  -> their_pub:lbuffer uint8 32ul
-  -> Stack bool
-    (requires fun h0 ->
-      Vale.X64.CPU_Features_s.(adx_enabled /\ bmi2_enabled) /\
-      live h0 shared /\ live h0 my_priv /\ live h0 their_pub /\
-      disjoint shared my_priv /\ disjoint shared their_pub)
-    (ensures  fun h0 r h1 -> modifies (loc shared) h0 h1 /\
-      as_seq h1 shared == Spec.Curve25519.scalarmult (as_seq h0 my_priv) (as_seq h0 their_pub)
-      /\ (not r == Lib.ByteSequence.lbytes_eq #32 (as_seq h1 shared) (Lib.Sequence.create 32 (u8 0))))
+val scalarmult: scalarmult_st M64
+val secret_to_public: secret_to_public_st M64
+val ecdh: ecdh_st M64
